test/correct_progs/out/task_id_18Tests.dfy
@@ -1,16 +1,16 @@
 // Auto-generated test cases by DafnyTestGen
 // Source: C:\Dados\Dafny\DafnyTestGen\test\correct_progs\in\task_id_18.dfy
 // Method: RemoveChars
-// Generated: 2026-04-17 19:30:39
+// Generated: 2026-04-17 20:09:40
 
 // Remove from the first string all characters which are present in the second string.
 // Preserves the order of the remaining elements.
 method RemoveChars(s1: string, s2: string) returns (v: string)
-  ensures v == Filter(s1, c => !(c in s2))
+  ensures v == Filter(s1, s2)
 {
   v := [];
   for i := 0 to |s1|
-    invariant v == Filter(s1[..i], c => !(c in s2))
+    invariant v == Filter(s1[..i], s2)
   {
     if !(s1[i] in s2) {
       v := v + [s1[i]];
@@ -21,12 +21,12 @@ method RemoveChars(s1: string, s2: string) returns (v: string)
 }
 
 // Filters a sequence using a predicate.
-// Returns a new sequence with the elements of s that satisfy the predicate p.
-function {:fuel 6} Filter<T>(s: seq<T>, p: T -> bool): (r : seq<T>)
+// Returns a new sequence with the elements of s that are not in t.
+function {:fuel 6} Filter<T(==)>(s: seq<T>, t: seq<T>): (r : seq<T>)
 {
     if |s| == 0 then []
-    else if p(s[|s|-1] ) then Filter(s[..|s|-1] , p) + [s[|s|-1] ]
-    else Filter(s[..|s|-1] , p)
+    else if s[|s|-1] !in t then Filter(s[..|s|-1] , t) + [s[|s|-1] ]
+    else Filter(s[..|s|-1] , t)
 }
 
 
@@ -45,9 +45,9 @@ method RemoveCharsTest(){
 method TestsForRemoveChars()
 {
   // Test case for combination {1}:
-  //   POST: v == Filter(s1, (c: char) => !(c in s2))
+  //   POST: v == Filter(s1, s2)
   //   POST: v == []
-  //   ENSURES: v == Filter(s1, (c: char) => !(c in s2))
+  //   ENSURES: v == Filter(s1, s2)
   {
     var s1: seq<char> := [];
     var s2: seq<char> := [];
@@ -57,8 +57,8 @@ method TestsForRemoveChars()
 
   // Test case for combination {2}:
   //   POST: !(|s1| == 0)
-  //   POST: v == if !(s1[|s1| - 1] in s2) then Filter<T>(s1[..|s1| - 1], (c: char) => !(c in s2)) + [s1[|s1| - 1]] else Filter<T>(s1[..|s1| - 1], (c: char) => !(c in s2))
-  //   ENSURES: v == Filter(s1, (c: char) => !(c in s2))
+  //   POST: v == if s1[|s1| - 1] !in s2 then Filter<T>(s1[..|s1| - 1], s2) + [s1[|s1| - 1]] else Filter<T>(s1[..|s1| - 1], s2)
+  //   ENSURES: v == Filter(s1, s2)
   {
     var s1: seq<char> := ['U'];
     var s2: seq<char> := ['U'];
@@ -67,9 +67,9 @@ method TestsForRemoveChars()
   }
 
   // Test case for combination {1}/O|s2|=1:
-  //   POST: v == Filter(s1, (c: char) => !(c in s2))
+  //   POST: v == Filter(s1, s2)
   //   POST: v == []
-  //   ENSURES: v == Filter(s1, (c: char) => !(c in s2))
+  //   ENSURES: v == Filter(s1, s2)
   {
     var s1: seq<char> := [];
     var s2: seq<char> := [' '];
@@ -78,9 +78,9 @@ method TestsForRemoveChars()
   }
 
   // Test case for combination {1}/O|s2|>=2:
-  //   POST: v == Filter(s1, (c: char) => !(c in s2))
+  //   POST: v == Filter(s1, s2)
   //   POST: v == []
-  //   ENSURES: v == Filter(s1, (c: char) => !(c in s2))
+  //   ENSURES: v == Filter(s1, s2)
   {
     var s1: seq<char> := [];
     var s2: seq<char> := [' ', '8'];
