test/correct_progs/out/task_id_401Tests.dfy
@@ -1,7 +1,7 @@
 // Auto-generated test cases by DafnyTestGen
 // Source: C:\Dados\Dafny\DafnyTestGen\test\correct_progs\in\task_id_401.dfy
 // Method: DeepElementWiseAddition
-// Generated: 2026-04-17 19:31:47
+// Generated: 2026-04-18 11:27:55
 
 method DeepElementWiseAddition(a: seq<seq<int>>, b: seq<seq<int>>) returns (result: seq<seq<int>>)
   requires |a| == |b| 
@@ -99,6 +99,22 @@ method TestsForDeepElementWiseAddition()
     expect result == [[]];
   }
 
+  // Test case for combination {1}/Q|a[0]|>=2:
+  //   PRE:  |a| == |b|
+  //   PRE:  forall i: int :: 0 <= i < |a| ==> |a[i]| == |b[i]|
+  //   POST: |result| == |a|
+  //   POST: forall i: int :: 0 <= i < |result| ==> IsElementWiseAddition(a[i], b[i], result[i])
+  //   ENSURES: |result| == |a|
+  //   ENSURES: forall i: int :: 0 <= i < |result| ==> IsElementWiseAddition(a[i], b[i], result[i])
+  {
+    var a: seq<seq<int>> := [[0, 37], [38], []];
+    var b: seq<seq<int>> := [[0, 39], [48], []];
+    var result := DeepElementWiseAddition(a, b);
+    expect |result| == |a|;
+    expect forall i: int :: 0 <= i < |result| ==> IsElementWiseAddition(a[i], b[i], result[i]);
+    expect result == [[0, 76], [86], []]; // observed from implementation
+  }
+
 }
 
 method TestsForElementWiseAddition()
@@ -140,6 +156,19 @@ method TestsForElementWiseAddition()
     var b: seq<int> := [];
     var result := ElementWiseAddition(a, b);
     expect result == [];
+  }
+
+  // Test case for combination {1}/R4:
+  //   PRE:  |a| == |b|
+  //   POST: IsElementWiseAddition(a, b, result)
+  //   POST: |a| == |b|
+  //   POST: forall i: int {:trigger b[i]} {:trigger a[i]} {:trigger result[i]} :: 0 <= i && i < |a| ==> result[i] == a[i] + b[i]
+  //   ENSURES: IsElementWiseAddition(a, b, result)
+  {
+    var a: seq<int> := [-2];
+    var b: seq<int> := [7721];
+    var result := ElementWiseAddition(a, b);
+    expect result == [7719];
   }
 
 }
